theories/L6_PCPS/closure_conversion_corresp.v
@@ -2,10 +2,9 @@
  * Author: Zoe Paraskevopoulou, 2016
  *)
 
-From CertiCoq.L6 Require Import cps cps_util set_util identifiers ctx hoare Ensembles_util
-               List_util functions logical_relations eval.
-Require Import CertiCoq.L6.closure_conversion CertiCoq.L6.closure_conversion_util.
-Require Import CertiCoq.L6.closure_conversion_correct.
+Require Import L6.closure_conversion L6.closure_conversion_util.
+From CertiCoq.L6 Require Import cps cps_util set_util identifiers ctx Ensembles_util
+     List_util functions logical_relations eval.
 Require Import compcert.lib.Coqlib.
 Require Import Coq.ZArith.Znumtheory Coq.Relations.Relations Coq.Arith.Wf_nat.
 Require Import Coq.Lists.List Coq.MSets.MSets Coq.MSets.MSetRBT Coq.Numbers.BinNums
@@ -17,8 +16,48 @@ Import ListNotations.
 Open Scope ctx_scope.
 Open Scope fun_scope.
 
-
 (** * Correspondence of the relational and the computational definitions of closure conversion *)
+
+
+(* Sketch of what we want to show: *)
+
+Lemma exp_closure_conv_Closure_conv_sound :
+  (forall e Scope Funs c Γ FVs FVmap S
+          (* The invariant that relates [FVmap] and [Scope], [Funs], [FV] *)
+          (Minv : FVmap_inv FVmap Scope Funs FVs)
+          (* [FVmap] contains all the free variables *)
+          (Hbin1 : binding_in_map (occurs_free e) FVmap)
+          (* [FVmap] does not contain the variables in [S] or [Γ] *)
+          (Hbin2 : binding_not_in_map (Union _ S (Singleton _ Γ)) FVmap)
+          (* [S] is disjoint with the free and bound variables of [e] and [Γ] *)
+          (HD1 : Disjoint _ S (Union _ (image (subst FVmap) (Setminus _ Funs Scope))
+                                     (Union _ (bound_var e)
+                                            (Union _ (occurs_free e) (Singleton _ Γ)))))
+          (* The current environment argument is fresh *)
+          (HD2 : ~ In _ (Union _ (bound_var e) (occurs_free e)) Γ),
+      {{ fun s => fresh S (next_var s) }}
+        exp_closure_conv clo_tag e FVmap Gmap c Γ
+        {{ fun s ef s' =>
+             exists C, is_exp_ctx (snd ef) C /\
+                       Closure_conversion clo_tag Scope Funs GFuns (subst FVmap) c Γ FVs e (fst ef) C /\
+                       fresh S (next_var s')
+  }}) /\
+  (forall B FVmap Funs FVs S c
+          (Minv : FVmap_inv FVmap (Empty_set _) Funs FVs)
+          (Hbin1 : binding_in_map (Union _ (occurs_free_fundefs B) (name_in_fundefs B)) FVmap)
+          (Hbin2 : binding_not_in_map S FVmap)
+          (HD1 : Disjoint _ S (Union _ (image (subst FVmap) Funs)
+                                     (Union _ (bound_var_fundefs B) (occurs_free_fundefs B))))
+          (Hinc : Included _ (name_in_fundefs B) Funs),
+      {{ fun s => fresh S (next_var s) }}
+        fundefs_closure_conv clo_tag B FVmap c
+        {{ fun s B' s' =>     
+             Closure_conversion_fundefs clo_tag Funs (subst FVmap) c FVs B B' /\
+             fresh S (next_var s')
+  }}).
+Proof with now eauto with Ensembles_DB functions_BD.
+
+
 
 Section CC_correct.
 
