theories/L6_PCPS/hoisting.v
@@ -3,7 +3,7 @@
  *)
 
 Require Import L6.cps L6.cps_util L6.identifiers L6.eval L6.env L6.ctx L6.size_cps
-        L6.logical_relations L6.Ensembles_util L6.List_util L6.map_util L6.tactics L6.bounds.
+        L6.logical_relations L6.Ensembles_util L6.List_util L6.map_util L6.tactics.
 Require Import compcert.lib.Coqlib.
 Require Import Coq.Lists.List Coq.NArith.BinNat Coq.Relations.Relations
         Coq.omega.Omega Coq.Sets.Ensembles Coq.Classes.Morphisms.
